LNSet.v
@@ -1,0 +1,77 @@
+(* ~~~~~~~~~~~~~~~~~~~~~~~~~~~~~~~~~~~~~~~~~~~~~~~~~~~~~~~~~~ *)
+(** * Notations for [Coq.Lists.ListSet] using the [EqDec] class.
+
+TODO: switch to using MSets in lieu of ListSet.
+*)
+(* ~~~~~~~~~~~~~~~~~~~~~~~~~~~~~~~~~~~~~~~~~~~~~~~~~~~~~~~~~~ *)
+(* [Coq.Classes.EquivDec] is Coq 8.3 only *)
+Require Import Coq.Lists.ListSet.
+Require Import Coq.Classes.EquivDec.
+
+(* ~~~~~~~~~~~~~~~~~~~~~~~~~~~~~~~~~~~~~~~~~~~~~~~~~~~~~~~~~~ *)
+Notation "\{}"          := (empty_set _)
+    : listset_scope.
+
+Notation "\{ x }"       := (set_add equiv_dec x (empty_set _))
+    : listset_scope.
+
+Notation "x \a ys"      := (set_add equiv_dec x ys)
+    (at level 37, right associativity) : listset_scope.
+
+Notation "xs \u ys"     := (set_union equiv_dec xs ys)
+    (at level 37, right associativity) : listset_scope.
+
+Notation "xs \n ys"     := (set_inter equiv_dec xs ys)
+    (at level 36, right associativity) : listset_scope.
+
+Notation "xs \\ ys"     := (set_diff equiv_dec xs ys)
+    (at level 34, left associativity) : listset_scope.
+
+Notation "xs \- y"      := (set_remove equiv_dec y xs)
+    (at level 34, left associativity) : listset_scope.
+
+Notation "x \in xs"     := (set_In x xs)
+    (at level 39) : listset_scope.
+
+Notation "x \notin xs"  := (~ set_In x xs)
+    (at level 39) : listset_scope.
+    (* Beware of unfolding issues with [not]. *)
+
+Delimit Scope listset_scope with set.
+Bind Scope listset_scope with set.
+Open Scope listset_scope.
+
+(* ~~~~~~~~~~~~~~~~~~~~~~~~~~~~~~~~~~~~~~~~~~~~~~~~~~~~~~~~~~ *)
+(*
+Definition Equal xs ys           := forall x:A, set_In x xs <-> set_In x ys.
+Definition Subset xs ys          := forall x:A, set_In x xs -> set_In x ys.
+Definition Inhab xs              := exists x:A, set_In x xs.
+Definition Empty xs              := forall x:A, ~ set_In x xs.
+Definition Disjoint xs ys        := forall x:A, ~ set_In x (xs \n ys).
+Definition Forall (P:A->Prop) xs := forall x:A, set_In x xs -> P x.
+Definition Exists (P:A->Prop) xs := exists x:A, set_In x xs /\ P x.
+
+Notation "xs [=] ys" := (Equal xs ys)
+    (at level 70, no associativity) : listset_scope.
+Notation "xs [<=] ys" := (Subset xs ys)
+    (at level 70, no associativity) : listset_scope.
+Notation "xs \c ys" := (Subset xs ys)
+    (at level 38) : listset_scope.
+
+Theorem set_In_classical
+    : forall {A : Type} (eq_dec : forall x y : A, {x = y} + {x <> y})
+    (x : A) (xs : set A), ~~set_In x xs -> set_In x xs.
+Proof.
+  intros A eq_dec x xs; induction xs as [|x0 xs0 IHxs0]; intro H;
+    [ apply H; intro H0; apply H0
+    | destruct (eq_dec x x0) as [L|R];
+      [ left; congruence
+      | right; apply IHxs0; intro H0; apply H; intro H1; destruct H1;
+        [ apply R; congruence
+        | apply H0; assumption ] ] ].
+Qed.
+Hint Resolve set_In_classical :sets.
+*)
+
+(* ~~~~~~~~~~~~~~~~~~~~~~~~~~~~~~~~~~~~~~~~~~~~~~~~~~~~~~~~~~ *)
+(* ~~~~~~~~~~~~~~~~~~~~~~~~~~~~~~~~~~~~~~~~~~~~~~~~~~~~~ fin. *)
