LNVar.v
@@ -1,0 +1,153 @@
+(* ~~~~~~~~~~~~~~~~~~~~~~~~~~~~~~~~~~~~~~~~~~~~~~~~~~~~~~~~~~ *)
+(** * Free variables/names for the locally nameless style.
+
+cf <http://www.chargueraud.org/viewcoq.php?sFile=softs%2Ftlc%2Fsrc%2FLibVar.v>
+*)
+(* ~~~~~~~~~~~~~~~~~~~~~~~~~~~~~~~~~~~~~~~~~~~~~~~~~~~~~~~~~~ *)
+(* [Coq.Classes.EquivDec] is Coq 8.3 only *)
+Require Import Coq.Arith.Lt.
+Require Import Coq.Arith.Plus.
+Require Import Coq.Arith.EqNat.
+Require Import Coq.Lists.ListSet.
+Require Import Coq.Lists.List.
+Require Import Coq.Classes.EquivDec.
+Require Import WrengrUtil.Tactics.Introv.
+Require Import WrengrUtil.CoqExtras.Nat.
+Require Export LNSet.
+
+(* ~~~~~~~~~~~~~~~~~~~~~~~~~~~~~~~~~~~~~~~~~~~~~~~~~~~~~~~~~~ *)
+(** * The specification of a variable type. *)
+Class VarType (Var : Set) `{eqdec0 : EqDec Var eq} :=
+    { inhabVar : inhabited Var
+    ; freshVar : forall (xs:set Var), { x:Var | x \notin xs }
+    }.
+
+
+(*
+(** * The specification of a variable type. *)
+Module Type VarType.
+
+    (** We leave the type of variables abstract. *)    
+    Parameter Var : Set.
+    
+    (** This type is inhabited. *) (* TODO: who cares? *)
+    Parameter inhabVar : inhabited Var.
+    
+    (** We can decide equality on this type. *)
+    Parameter _VarEqDec : EqDec Var eq. (* Defines [equiv_dec] *)
+    Program Instance VarEqDec : EqDec Var eq := _VarEqDec.
+    
+    (** Finally, we have a means of generating fresh variables. *)
+    Parameter freshVar : forall (xs:set Var), { x:Var | x \notin xs }.
+
+End VarType.
+*)
+
+
+(* ~~~~~~~~~~~~~~~~~~~~~~~~~~~~~~~~~~~~~~~~~~~~~~~~~~~~~~~~~~ *)
+(** * A concrete implementation using [nat]. *)
+
+(* Module Export NatVar : VarType. *)
+Section NatVar.
+
+    Definition NatVar := nat.
+
+    Lemma inhabNatVar : inhabited NatVar.
+    Proof. apply inhabits. apply 0. Qed.
+    
+    Program Instance NatVarEqDec : EqDec NatVar eq := nat_eq_eqdec.
+    
+    (** The method for generating a new variable. *)
+    Definition genNatVar (xs:set NatVar) : NatVar :=
+        1 + fold_right plus 0 xs.
+    
+    (** A lemma for proving [freshNatVar_spec]. *)
+    Lemma genNatVar_gt : forall xs x, x \in xs -> x < genNatVar xs.
+    Proof.
+      unfold genNatVar. induction xs as [ | x0 xs0 IHxs0 ]; introv I.
+        contradiction.
+        
+        destruct I as [H | I']; simpl.
+          rewrite H.
+          auto with arith.
+          (* Or:
+          rewrite plus_Snm_Sn_m.
+          apply lt_plus_trans.
+          apply lt_n_Sn.
+          *)
+          
+          simpl in IHxs0.
+          (* [auto with arith] can's solve any part of this. Is the [plus_Snm_n_Sm] hint really in there?? *)
+          rewrite plus_Snm_n_Sm.
+          rewrite plus_comm.
+          apply lt_plus_trans.
+          apply IHxs0.
+          exact I'.
+    Qed.
+    
+    (** Proof that [genNatVar] satisfies the specification of [freshNatVar]. *)
+    Lemma freshNatVar_spec : forall xs, (genNatVar xs) \notin xs.
+    Proof.
+      unfold genNatVar, not. intros xs H.
+      destruct xs as [|x0 xs0]; simpl.
+        assumption.
+        
+        inversion_clear H as [H0|H0]; simpl in H0.
+          rewrite plus_comm in H0.
+          exact (succ_plus_discr _ _ H0).
+          
+          apply genNatVar_gt    in H0.
+          unfold genNatVar      in H0.
+          rewrite plus_Snm_n_Sm in H0.
+          destruct x0.
+            exact (lt_irrefl _ H0).
+            
+            assert (H1 : forall x y, ~ S x + y < y) by auto with arith.
+            exact (H1 _ _ H0).
+    Qed.
+    
+    Lemma freshNatVar : forall (xs:set NatVar), { x:NatVar | x \notin xs }.
+    Proof. intros xs. exists (genNatVar xs). apply freshNatVar_spec. Qed.
+
+    Instance NatVarType : VarType NatVar :=
+        { inhabVar := inhabNatVar
+        ; freshVar := freshNatVar
+        }.
+End NatVar.
+
+
+(* ~~~~~~~~~~~~~~~~~~~~~~~~~~~~~~~~~~~~~~~~~~~~~~~~~~~~~~~~~~ *)
+(* N.B., must use a section in order to use [Context], and must use
+    [Context] instead of [Variable] if we want it to be implicit.
+    However, we can't define notations inside sections if we want
+    them to last. *)
+Section DerivedOperations.
+Context  {Var : Set}.
+Context `{VT : VarType Var}.
+
+
+(** Freshness of [n] variables [ys] from a set [xs] and from one another. *)
+Fixpoint Fresh (xs:set Var) (n:nat) (ys:set Var) {struct ys} : Prop :=
+    match ys, n with
+    | nil,    O    => True
+    | y::ys', S n' => y \notin xs /\ Fresh (y \a xs) n' ys'
+    | _,      _    => False
+    end.
+(* TODO: How is this different than [Hint Unfold Fresh]? *)
+Hint Extern 1 (Fresh _ _ _) => simpl.
+
+
+(** Generate [n] variables fresh from [xs] and one another. *)
+Lemma freshVars : forall xs n, { ys:set Var | Fresh xs n ys }.
+Proof.
+  intros. generalize dependent xs. induction n; intros xs;
+    [ exists nil; auto
+    | destruct (freshVar xs)   as [y  Hy]
+    ; destruct (IHn (y \a xs)) as [ys Hys]
+    ; exists (y::ys); auto
+    ].
+Qed.
+End DerivedOperations.
+
+(* ~~~~~~~~~~~~~~~~~~~~~~~~~~~~~~~~~~~~~~~~~~~~~~~~~~~~~~~~~~ *)
+(* ~~~~~~~~~~~~~~~~~~~~~~~~~~~~~~~~~~~~~~~~~~~~~~~~~~~~~ fin. *)
